readme and clean up

src/semantics/completeness.lean
@@ -1,7 +1,3 @@
-/-
-Copyright (c) 2021 Paula Neeley. All rights reserved.
-Author: Paula Neeley
--/
 
 import semantics.consistency syntax.soundness
 
@@ -9,37 +5,56 @@ local attribute [instance] classical.prop_decidable
 
 open  Kproof
 
----------------------- Canonical Model Construction ----------------------
+/-
+
+In this file we prove completeness (found near the end of the file) for
+K modal logic.
+
+The classic proof goes like this utilizes a canonical model for K. In other words,
+a modal model where the worlds are sets of formulas such that whenever there is 
+a set Γ that is consistent, there also a exists a world for it. Furthermore, 
+the accesibility relation and valuation function are defined such that truth
+in a world and membership in one of the worlds are the same thing. 
+
+The big helper functions needed are to prove Lindenbaum's lemma, which states
+that a set of formulas Γ is complete iff for every formula A, we have at least 
+one of A ∈ Γ or ¬A ∈ Γ. This is proved in consistency.#check
+
+Another helper function that is important is the Truth lemma, such that whenever
+a world in the canonical model satisfies a formula, that formula is in the 
+world itself (because recall the worlds are sets of formulas). 
+
+-/
 
 namespace canonical
 
 
-def canonical (AX : ctx) [hax : sem_cons AX] : frame := 
+def canonical (Γ : ctx) [hax : sem_cons Γ] : frame := 
 { 
-  W := {xΓ : ctx // max_ax_consist AX xΓ},
+  W := {xΓ : ctx // max_ax_consist Γ xΓ},
   W_inhabited := 
   begin 
-    have h1 := max_ax_exists AX hax, 
+    have h1 := max_ax_exists Γ hax, 
     choose Γ h1 using h1, 
-    exact ⟨⟨Γ, h1⟩⟩ 
+    exact subtype.inhabited h1,
   end,
   R := λ xΓ yΔ, ∀ A : form, □A ∈ xΓ.val → A ∈ yΔ.val
 }
 
 
-def val_canonical (AX : ctx) [hax : sem_cons AX] : nat → (canonical AX).W → Prop :=
-  λ n, λ xΓ : (canonical AX).W, (p n) ∈ xΓ.val
+def val_canonical (Γ : ctx) [hax : sem_cons Γ] : nat → (canonical Γ).W → Prop :=
+  λ n, λ xΓ : (canonical Γ).W, (p n) ∈ xΓ.val
 
 
-lemma existence (AX : ctx) (hax : sem_cons AX) (xΓ : (canonical AX).W) :
-  ∀ A, ◇A ∈ xΓ.val ↔ ∃ yΔ : (canonical AX).W, A ∈ yΔ.val ∧ (canonical AX).R xΓ yΔ :=
+lemma existence (Γ : ctx) (hax : sem_cons Γ) (xΓ : (canonical Γ).W) :
+  ∀ A, ◇A ∈ xΓ.val ↔ ∃ yΔ : (canonical Γ).W, A ∈ yΔ.val ∧ (canonical Γ).R xΓ yΔ :=
 begin
 intro A, split,
 intro h1,
 let Γbox : ctx := {B : form | □B ∈ xΓ.val},
-have h1 : ax_consist AX (Γbox ∪ {A}), 
+have h1 : ax_consist Γ (Γbox ∪ {A}), 
 {by_contradiction h2, simp at h2,
-have h3 := five AX Γbox A h2,
+have h3 := five Γ Γbox A h2,
 cases h3 with L h3, cases h3 with h3 h4,
 have h5 := cut fin_conj_boxn (mp kdist (nec h4)),
 have h6 := exercise1,
@@ -48,14 +63,14 @@ intros B h8, simp at *, cases h8 with a h8,
 cases h8 with h8l h8r,
 subst h8r, exact h3 a h8l,
 specialize h6 xΓ.2 h7 h5,
-have h8 := (six AX xΓ.1 (max_imp_ax xΓ.2)).mp xΓ.2 (¬A).box,
+have h8 := (six Γ xΓ.1 (max_imp_ax xΓ.2)).mp xΓ.2 (¬A).box,
 cases h8 with h8l h8r, simp at *,
 exact absurd h1 (h8r h6)
 },
-have h2 := lindenbaum AX (Γbox ∪ {A}) h1,
+have h2 := lindenbaum Γ (Γbox ∪ {A}) h1,
 cases h2 with Δ h2, cases h2 with h2 h3,
-let xΔ : (canonical AX).W := ⟨Δ, h2⟩,
-existsi (xΔ : (canonical AX).W),
+let xΔ : (canonical Γ).W := ⟨Δ, h2⟩,
+existsi (xΔ : (canonical Γ).W),
 have h5 := set.union_subset_iff.mp h3,
 cases h5, split, simp at h5_right, exact h5_right,
 have h3 : ∀ A : form, □A ∈ xΓ.val → A ∈ xΔ.val,
@@ -64,15 +79,15 @@ exact h3,
 simp at *,
 intros yΔ h1 h2,
 by_contradiction h3,
-have h4 := (max_notiff AX xΓ.1 xΓ.2 (◇A)).mp h3,
-have h5 := (max_dn AX xΓ.1 xΓ.2 (□¬A)).mpr h4,
-have h6 := (max_notiff AX yΔ.1 yΔ.2 A).mpr (h2 (¬A) h5),
+have h4 := (max_notiff Γ xΓ.1 xΓ.2 (◇A)).mp h3,
+have h5 := (max_dn Γ xΓ.1 xΓ.2 (□¬A)).mpr h4,
+have h6 := (max_notiff Γ yΔ.1 yΔ.2 A).mpr (h2 (¬A) h5),
 exact absurd h1 h6
 end
 
 
-lemma truth (AX : ctx) (hax : sem_cons AX) (xΓ : (canonical AX).W) : 
-  ∀ A, true_at_world (canonical AX) (val_canonical AX) xΓ A ↔ (A ∈ xΓ.val) :=
+lemma truth (Γ : ctx) (hax : sem_cons Γ) (xΓ : (canonical Γ).W) : 
+  ∀ A, true_at_world (canonical Γ) (val_canonical Γ) xΓ A ↔ (A ∈ xΓ.val) :=
 begin
 intro A, induction A with n A B ih_A ih_B 
 A B ih_A ih_B A ih_A generalizing xΓ,
@@ -99,10 +114,10 @@ apply (ih_B xΓ).mpr,
 exact max_imp_2 xΓ.2 h1 ((ih_A xΓ).mp h2),
 split, intros h1, 
 by_contradiction h2,
-have h4 := (existence AX hax xΓ (¬A)).mp,
-have h5 := max_boxdn AX xΓ.1 xΓ.2 A ((max_notiff AX xΓ.1 xΓ.2 A.box).mp h2),
+have h4 := (existence Γ hax xΓ (¬A)).mp,
+have h5 := max_boxdn Γ xΓ.1 xΓ.2 A ((max_notiff Γ xΓ.1 xΓ.2 A.box).mp h2),
 cases h4 h5 with xΔ h4, cases h4 with h4 h6,
-have h7 := max_notiff AX xΔ.1 xΔ.2 A,
+have h7 := max_notiff Γ xΔ.1 xΔ.2 A,
 cases h7 with h7l h7r,
 exact absurd ((ih_A xΔ).mp (h1 xΔ h6)) (h7r h4),
 intros h1 xΔ h2,
@@ -110,14 +125,14 @@ apply (ih_A xΔ).mpr, exact h2 A h1,
 end
 
 
-lemma comphelper (AX : ctx) (A : form) (hax : sem_cons AX) : 
-  ¬  Kproof AX A → ax_consist AX {¬A} :=
+lemma comphelper (Γ : ctx) (A : form) (hax : sem_cons Γ) : 
+  ¬  Kproof Γ A → ax_consist Γ {¬A} :=
 begin
 intro h1, intros L h2,
 rw fin_ax_consist, induction L,
 by_contradiction h3,
-exact absurd (mp dne h3) (nprfalse AX hax), 
-have h4 : (∀ B ∈ L_hd::L_tl, B = ¬A) →  Kproof AX (¬fin_conj (L_hd::L_tl)) →  Kproof AX A, 
+exact absurd (mp dne h3) (nprfalse Γ hax), 
+have h4 : (∀ B ∈ L_hd::L_tl, B = ¬A) →  Kproof Γ (¬fin_conj (L_hd::L_tl)) →  Kproof Γ A, 
 from fin_conj_repeat hax,
 simp at *, 
 cases h2 with h2 h3,
@@ -127,36 +142,37 @@ exact h6
 end 
 
 
-theorem forcesAX (AX : ctx) (hax : sem_cons AX) : 
-  ctx_true_in_model (canonical AX) (val_canonical AX) AX :=
+theorem forcesΓ (Γ : ctx) (hax : sem_cons Γ) : 
+  ctx_true_in_model (canonical Γ) (val_canonical Γ) Γ :=
 begin
 intros A xΓ h1,
 have h2 : ∀ B ∈ list.nil, B ∈ xΓ.val, 
 {intros B h3, have h4 := list.ne_nil_of_length_pos (list.length_pos_of_mem h3),
 simp at *, exact false.elim h4},
-exact (truth AX hax xΓ A).mpr (exercise1 xΓ.2 h2 (mp pl1 (ax h1)))
+exact (truth Γ hax xΓ A).mpr (exercise1 xΓ.2 h2 (mp pl1 (ax h1)))
 end
 
 
-theorem completeness (AX : ctx) (hax : sem_cons AX) (A : form) : 
-  entails AX A →  Kproof AX A :=
+theorem completeness (Γ : ctx) (hax : sem_cons Γ) (A : form) : 
+  entails Γ A →  Kproof Γ A :=
 begin
-rw ←not_imp_not, intro h1,
-have h2 := comphelper AX A hax h1,
-have h3 := lindenbaum AX {¬A} h2,
+rw ←not_imp_not, 
+intro h1,
+have h2 := comphelper Γ A hax h1,
+have h3 := lindenbaum Γ {¬A} h2,
 simp at *,
 cases h3 with Γ' h3, cases h3 with h3 h4, 
 rw entails, 
 push_neg,
-let f := canonical, use f AX,
-let v := val_canonical, use v AX,
-let xΓ' : (f AX).W := ⟨Γ', h3⟩,
+let f := canonical, use f Γ,
+let v := val_canonical, use v Γ,
+let xΓ' : (f Γ).W := ⟨Γ', h3⟩,
 split, 
-exact forcesAX AX hax,
+exact forcesΓ Γ hax,
 use xΓ',
-have h5 := truth AX hax xΓ' ¬A,
+have h5 := truth Γ hax xΓ' ¬A,
 cases h5 with h5 h6,
-have h7 := not_forces_imp (f AX) (v AX) xΓ' A,
+have h7 := not_forces_imp (f Γ) (v Γ) xΓ' A,
 cases h7 with h7 h8, apply h8, apply h6, exact h4
 end
 
