src/syntax/syntax.lean
@@ -1,11 +1,21 @@
 
 
-/- SYNTΓ -/
+--------------------------------------------------------------------------------
+/- SYNTAX -/
+--------------------------------------------------------------------------------
 
 /-
 
-In our aim to formalize modal logic, we will aim to implement a deep embedding.
-The first step in this is to formalize the syntax of modal logic in lean.
+In our aim to formalize modal logic, we first need to capture its syntax. 
+To do this, we'll implement a deep embedding in Lean.
+
+-/
+
+--------------------------------------------------------------------------------
+
+/- 
+
+§ Formulas
 
 We will aim to define formulas reflecting the classical definition i.e. 
 
@@ -23,12 +33,15 @@ We will aim to define formulas reflecting the classical definition i.e.
     - '◇ A'
 7. Nothing else is a formula
 
-This is an inductive definition, so we'll define these formulas
-in Lean similarly.
-
-Specifically, we'll encode '⊥' as 'bot' (and let '⊤' be its negation).#check
-
-Since each sentence symbol is indexed, it will take an index argument.#check
+This is an inductive definition, so we'll define these formulas 
+in Lean similarly. Furthermore, we'll define only a select amount of these 
+formulas, namely:
+- '⊥' as "bot"
+- sentence symbols 'pᵢ' as "var" + a natural number to identify them
+- '∧' as "and", and will be denoted in Lean as "&"
+- '→' as "impl" 
+- '□' as "box"
+The other formulas can be defined in terms of these basic ones.
 
 -/
 
@@ -52,26 +65,72 @@ notation A `↔` B := (A ⊃ B) & (B ⊃ A)
 notation `□`:80  := form.box 
 notation `◇`:80  := λ A, ¬(□(¬A))
 
----------------------- Proof System ----------------------
+--------------------------------------------------------------------------------
+
+/-
+
+§ Proof system
+
+Here we define the proof system of K for modal logic. K is nice
+because it is the smallest normal modal logic, which gives us nice features
+such as completeness and soundness. The proof system itself is used to reason
+about the syntax of the language: it is a set of rules about how to syntactially
+"get" new formulas and make reasonings. Later on, we'll define the semantics
+of modal logic which deals with meaning.
+
+We say that there is a modal derivation (a proof in K) from a 
+set of axioms (also referred to as the context) if there is a finite sequence
+of formulas such that each formula B meets one of the following conditions:
+
+1) B is an instance of a tautology
+
+2) B is an instance of some axiom in the ctx
+
+3) B follows by *modus ponens* of two earlier formulas 
+  - i.e. both 'A' and 'A → B' occur in the ctx
+
+4) B follows by *necessitation* of some prior formula
+  - i.e. given that 'A' occurs earlier, let 
+    B := □ A
+
+-/
 
 -- Define a context
 @[reducible] def ctx : Type := set (form)
 notation Γ `∪` A := set.insert A Γ
 
-
 -- Proof system
 inductive Kproof : ctx → form → Prop 
-| ax {Γ} {A} (h : A ∈ Γ) : Kproof Γ A
-| pl1 {Γ} {A B}           : Kproof Γ (A ⊃ (B ⊃ A))
-| pl2 {Γ} {A B χ}         : Kproof Γ ((A ⊃ (B ⊃ χ)) ⊃ ((A ⊃ B) ⊃ (A ⊃ χ)))
+| ax {Γ} {A} (h : A ∈ Γ) : Kproof Γ A                               -- axiom in ctx
+| pl1 {Γ} {A B}           : Kproof Γ (A ⊃ (B ⊃ A))                  -- tautologies
+| pl2 {Γ} {A B C}         : Kproof Γ ((A ⊃ (B ⊃ C)) ⊃ ((A ⊃ B) ⊃ (A ⊃ C)))
 | pl3 {Γ} {A B}           : Kproof Γ (((¬A) ⊃ (¬B)) ⊃ (((¬A) ⊃ B) ⊃ A))
 | pl4 {Γ} {A B}           : Kproof Γ (A ⊃ (B ⊃ (A & B)))
 | pl5 {Γ} {A B}           : Kproof Γ ((A & B) ⊃ A)
 | pl6 {Γ} {A B}           : Kproof Γ ((A & B) ⊃ B)
 | pl7 {Γ} {A B}           : Kproof Γ (((¬A) ⊃ (¬B)) ⊃ (B ⊃ A))
-| kdist {Γ} {A B}         : Kproof Γ ((□ (A ⊃ B)) ⊃ ((□ A) ⊃ (□ B)))
-| mp {Γ} {A B} 
+| kdist {Γ} {A B}         : Kproof Γ ((□ (A ⊃ B)) ⊃ ((□ A) ⊃ (□ B))) -- rule K 
+| mp {Γ} {A B}                                                       -- modus ponens
   (hpq: Kproof Γ (A ⊃ B)) 
   (hp : Kproof Γ A)         : Kproof Γ B
-| nec {Γ} {A} 
+| nec {Γ} {A}                                                        -- necessitation
   (hp: Kproof Γ A)          : Kproof Γ (□ A)
+
+  /-
+
+  Note that we hard coded some tautologies. This is because there are an 
+  infinite amount of tautologies; having to prove each instance as a lemma would 
+  be tedious. The following are tautologies that are hard coded:
+
+  1) A → B → A
+  2) (A → (B → C)) → ((A → B) → C)
+  3) (¬A → ¬B) → ((¬A → B) → A) 
+  4) A → (B → (A ∧ B))
+  5) (A ∧ B) → A
+  6) (A ∧ B) → B
+  7) (¬A → ¬B) → (B → A)
+
+  and an important one for modal logics, named K after Saul Kripke, 
+  - □(A → B) → (□A → □B)
+
+  -/
